MonadicHHL/HHLSyntax.lean
@@ -1,0 +1,325 @@
+import MonadicHHL.HHLMonads
+
+def H.type (M : Type _ → Type _) [Monad M] [HHL M] (α : Type _) : Type _ :=
+  @HHL.hyperassertion M _ _ α
+
+def H.pure {M : Type _ → Type _} [Monad M] [HHL M] {α : Type _} (P : Prop)
+  : H.type M α :=
+  fun _ => P
+
+class HHLSyntax (M : Type _ → Type _) [Monad M] extends HHL M where
+  -- Forall {α : Type _} (P : α → H.type M α) : H.type M α
+  -- Exists {α : Type _} (P : α → H.type M α) : H.type M α
+  -- Forall {α : Type _} (P : α → H.type M α) : H.type M α
+  --ForallActive {α : Type _} (b : α → Prop) (P : elemType α → H.type M α) : H.type M α
+  CheckElem {α : Type _} (b : α → Prop) (σ : elemType α) : Prop
+  MapElem {α β : Type _} (f : α → β) (σ : elemType α) : elemType β
+
+/-
+def H.low {M : Type _ → Type _} [Monad M] [HHLSyntax M] {α β : Type _}
+  (f : α → β) : H.type M α :=
+  HHLSyntax.Forall M (fun σ₁ => HHLSyntax.Forall M (fun σ₂ => H.pure (f σ₁ = f σ₂)))
+-/
+instance : HHLSyntax Id where
+  -- Forall P := fun S => ∀ σ ∈ S, P σ S
+  -- ForallActive b P := fun S => ∀ σ ∈ S, b σ → P σ S
+  CheckElem b σ := b σ
+  MapElem f := f
+
+instance : HHLSyntax Set where
+  -- Forall P := fun S => ∀ σ ∈ S, P σ S
+  -- ForallActive b P := fun S => ∀ σ ∈ S, b σ → P σ S
+  CheckElem b σ := b σ
+  MapElem f := f
+
+instance (M : Type _ → Type _) [Monad M] [LawfulMonad M] [HHLSyntax M] : HHLSyntax (OptionT M) where
+  /-
+  Forall P := HHLSyntax.Forall
+    (fun σ => match σ with
+      | some a => P a
+      | none   => H.pure True)
+  -/
+  CheckElem b := HHLSyntax.CheckElem (fun x => match x with
+      | some a => b a
+      | none   => False)
+  MapElem f := HHLSyntax.MapElem (fun x => match x with
+      | some a => some (f a)
+      | none   => none)
+
+def OptionT.isOk {α : Type _} {M : Type _ → Type _} [Monad M] [HHLSyntax M]
+  : HHL.elemType M (Option α) → Prop :=
+  HHLSyntax.CheckElem (fun x => Option.isSome x = true)
+
+def OptionT.isErr {α : Type _} {M : Type _ → Type _} [Monad M] [HHLSyntax M]
+  : HHL.elemType M (Option α) → Prop :=
+  HHLSyntax.CheckElem (fun x => match x with
+      | some _ => False
+      | none   => True)
+
+instance {σ : Type _} (M : Type _ → Type _) [Monad M] [LawfulMonad M] [HHLSyntax M]
+  : HHLSyntax (StateT σ M) where
+  -- Forall P := HHLSyntax.Forall (fun p => P p.1)
+  CheckElem b := HHLSyntax.CheckElem (fun p => b p.1)
+  MapElem f := HHLSyntax.MapElem (fun p => (f p.1, p.2))
+
+-- Concrete cases
+
+def Id.Forall {α : Type _} (P : α → H.type Id α) : H.type Id α :=
+  fun S => ∀ v ∈ S, P v S
+
+def Set.Forall {α : Type _} (P : α → H.type Set α) : H.type Set α :=
+  fun S => ∀ v ∈ S, P v S
+
+def OptionT.Id.ForallOk {α : Type _} (P : α → H.type (OptionT Id) α) : H.type (OptionT Id) α :=
+  fun S => ∀ v ∈ S,
+    match v with
+    | some x => P x S
+    | none   => True -- exists would be false
+
+def OptionT.Set.ForallOk {α : Type _} (P : α → H.type (OptionT Set) α)
+  : H.type (OptionT Set) α :=
+  fun S => ∀ v ∈ S,
+    match v with
+    | some x => P x S
+    | none   => True -- exists would be false
+
+def OptionT.Id.ForallErr {α : Type _} (P : Unit → H.type (OptionT Id) α) : H.type (OptionT Id) α :=
+  fun S => ∀ v ∈ S,
+    match v with
+    | some _ => True -- exists would be false
+    | none   => P () S
+
+def OptionT.Set.ForallErr {α : Type _} (P : Unit → H.type (OptionT Set) α)
+  : H.type (OptionT Set) α :=
+  fun S => ∀ v ∈ S,
+    match v with
+    | some _ => True -- exists would be false
+    | none   => P () S
+
+def StateT.Id.Forall {σ α : Type _} (P : α × σ → H.type (StateT σ Id) α)
+  : H.type (StateT σ Id) α :=
+  fun S => ∀ p ∈ S, P p S
+
+def StateT.Set.Forall {σ α : Type _} (P : α × σ → H.type (StateT σ Id) α)
+  : H.type (StateT σ Id) α :=
+  fun S => ∀ p ∈ S, P p S
+
+def OptionT.StateT.Id.ForallOk {σ α : Type _} (P : α × σ → H.type (OptionT (StateT σ Id)) α)
+  : H.type (OptionT (StateT σ Id)) α :=
+  fun S => ∀ p, p ∈ S → ∀ h : p.1.isSome, P (p.1.get h, p.2) S
+
+def OptionT.StateT.Id.ForallErr {σ α : Type _} (P : Unit × σ → H.type (OptionT (StateT σ Id)) α)
+  : H.type (OptionT (StateT σ Id)) α :=
+  fun S => ∀ p ∈ S, p.1.isNone → P ((), p.2) S
+
+-- How to turn x : ElemType M (Option α) into ElemType M α???
+-- Need a map elemType?
+
+-- How to write OptionT.StateT.Id.Forall with the combinators?
+def OptionT.ForallErr {α : Type _} {M : Type _ → Type _} [Monad M] [HHLSyntax M] [LawfulMonad M]
+  [Inhabited α]
+  (P : HHL.elemType M Unit → H.type (OptionT M) α) : H.type (OptionT M) α :=
+  (fun S =>
+    ∀ p ∈ S, OptionT.isErr p →
+    -- HHLSyntax.CheckElem (M := OptionT M) Option.isSome p →
+      P (HHLSyntax.MapElem (fun _ => ()) p) S)
+
+def OptionT.ForallOk {α : Type _} {M : Type _ → Type _} [Monad M] [HHLSyntax M] [LawfulMonad M]
+  [Inhabited α]
+  (P : HHL.elemType M α → H.type (OptionT M) α) : H.type (OptionT M) α :=
+  (fun S =>
+    ∀ p ∈ S, OptionT.isOk p →
+      P (HHLSyntax.MapElem the p) S)
+
+lemma forallOkState_same
+  {σ α : Type _}
+  [Inhabited α]
+  (P : α × σ → H.type (OptionT (StateT σ Id)) α) :
+  OptionT.StateT.Id.ForallOk P = OptionT.ForallOk P
+:= by
+  apply funext
+  intro S
+  simp [OptionT.StateT.Id.ForallOk, OptionT.ForallOk]
+  simp [HHLSyntax.MapElem]
+  simp [OptionT.isOk]
+  simp [HHLSyntax.CheckElem, the, Option.getD]
+  grind
+
+lemma forallErrState_same
+  {σ α : Type _}
+  [Inhabited α]
+  (P : Unit × σ → H.type (OptionT (StateT σ Id)) α) :
+  OptionT.StateT.Id.ForallErr P = OptionT.ForallErr P
+:= by
+  apply funext
+  intro S
+  simp [OptionT.StateT.Id.ForallErr, OptionT.ForallErr]
+  simp [HHLSyntax.MapElem]
+  simp [OptionT.isErr]
+  simp [HHLSyntax.CheckElem]
+  grind
+
+
+
+lemma forallOkId_same
+  {α : Type _}
+  [Inhabited α]
+  (P : α → H.type (OptionT Id) α) :
+  OptionT.Id.ForallOk P = OptionT.ForallOk P
+:= by
+  apply funext
+  intro S
+  simp [OptionT.Id.ForallOk, OptionT.ForallOk]
+  simp [HHLSyntax.MapElem]
+  simp [OptionT.isOk]
+  simp [HHLSyntax.CheckElem, the, Option.getD]
+  grind
+
+lemma forallErrId_same
+  {α : Type _}
+  [Inhabited α]
+  (P : Unit → H.type (OptionT Id) α) :
+  OptionT.Id.ForallErr P = OptionT.ForallErr P
+:= by
+  apply funext
+  intro S
+  simp [OptionT.Id.ForallErr, OptionT.ForallErr]
+  simp [HHLSyntax.MapElem]
+  simp [OptionT.isErr]
+  simp [HHLSyntax.CheckElem]
+  grind
+
+lemma forallOkSet_same
+  {α : Type _}
+  [Inhabited α]
+  (P : α → H.type (OptionT Set) α) :
+  OptionT.Set.ForallOk P = OptionT.ForallOk P
+:= by
+  apply funext
+  intro S
+  simp [OptionT.Set.ForallOk, OptionT.ForallOk]
+  simp [HHLSyntax.MapElem]
+  simp [OptionT.isOk]
+  simp [HHLSyntax.CheckElem, the, Option.getD]
+  grind
+
+lemma forallErrSet_same
+  {α : Type _}
+  [Inhabited α]
+  (P : Unit → H.type (OptionT Set) α) :
+  OptionT.Set.ForallErr P = OptionT.ForallErr P
+:= by
+  apply funext
+  intro S
+  simp [OptionT.Set.ForallErr, OptionT.ForallErr]
+  simp [HHLSyntax.MapElem]
+  simp [OptionT.isErr]
+  simp [HHLSyntax.CheckElem]
+  grind
+
+
+
+-- Let's pretend Option base is DivM
+
+instance : HHL Option where
+  elemType α := Option α
+  relWith {α β : Type _} (C : α → Option β) (p : Option α) (p' : Option β) :=
+    Option.bind p C = p'
+  bind_rel C₁ C₂ p₀ p₂ := by
+    simp [bind, Option.bind]
+    aesop
+
+instance : HHLSyntax Option where
+  -- Forall P := fun S => ∀ σ ∈ S, P σ S
+  CheckElem b σ :=
+    match σ with
+      | some a => b a
+      | none   => False
+  MapElem := Option.map
+
+
+abbrev DivMonad σ := OptionT (StateT σ Option)
+
+-- TODO
+
+example (σ : Type) : HHL.elemType (DivMonad σ) α = Option (Option α × σ) := by
+  simp [HHL.elemType]
+
+
+def ForallNonTerm {σ : Type _} {α : Type _} [Inhabited α]
+  (P : Unit → H.type (DivMonad σ) α) : H.type (DivMonad σ) α := fun S =>
+    ∀ p ∈ S, if p.isNone then P () S else True
+
+-- OptionT.ForallErr boils down Option (Unit × σ)
+-- OptionT.ForallOk boils down Option (α × σ)
+-- So need to check that it's some (otherwise it's clearly a NonTerm)
+
+def ForallErr {σ : Type _} {α : Type _} [Inhabited α]
+  (P : Unit × σ → H.type (DivMonad σ) α) : H.type (DivMonad σ) α := fun S =>
+  sorry
+
+/-
+
+lemma forall_optionT_Id_equiv
+  {α : Type _} (P : α → Prop) :
+  @HHLSyntax.Forall (OptionT Id) _ _ _ (fun σ => H.pure (P σ))
+  = (fun S => ∀ σ ∈ S, ∀ x, σ = Option.some x → P x) := by
+    apply funext
+    intro S
+    simp [HHLSyntax.Forall]
+    unfold H.pure
+    apply Iff.intro
+    {
+      intro h σ hσ x heq
+      specialize h (some x)
+      aesop
+    }
+    {
+      aesop
+    }
+
+def ForallState {σ : Type _} {M : Type _ → Type _} [Monad M] [HHLSyntax M] {α : Type _}
+  (P : α × σ → H.type M (α × σ)) : H.type (StateT σ M) α :=
+  @HHLSyntax.Forall M _ _ _ P
+
+lemma equiv_forall_state {σ α : Type _}
+  (P : α × σ → H.type Id (α × σ)) :
+  ForallState P
+  = (fun S => ∀ p ∈ S, P p S) := by
+  rfl
+
+abbrev StateOption (σ : Type _) : Type _ → Type _ := OptionT (StateT σ Id)
+
+lemma equiv_forall_state_option {σ α : Type _}
+  (P : α × σ → H.type (StateOption σ) α) :
+  @ForallState σ (StateOption σ) _ _ _ P
+  = sorry :=
+  sorry
+
+-/
+
+/-
+class HHL (M : Type _ → Type _) [Monad M] where
+  elemType (α : Type _) : Type _
+  relWith : {α β : Type _} → (α → M β) → elemType α → elemType β → Prop
+  bind_rel
+    {α₀ α₁ α₂ : Type _}
+    (C₁ : α₀ → M α₁) (C₂ : α₁ → M α₂)
+    (p₀ : elemType α₀) (p₂ : elemType α₂) :
+      relWith (fun v₁ ↦ bind (C₁ v₁) C₂) p₀ p₂
+      ↔ ∃ p₁, relWith C₁ p₀ p₁ ∧ relWith C₂ p₁ p₂
+-/
+
+def H.ForallActive {M : Type _ → Type _} [Monad M] [HHLSyntax M] {α : Type _}
+  (b : α → Prop) (P : HHL.elemType M α → H.type M α) : H.type M α :=
+  fun S => ∀ σ ∈ S, HHLSyntax.CheckElem b σ → P σ S
+
+-- generic (kinda useless) forall?
+def H.Forall {M : Type _ → Type _} [Monad M] [HHL M] {α : Type _}
+  (P : HHL.elemType M α → H.type M α) : H.type M α :=
+  fun S => ∀ σ ∈ S, P σ S
+
+def H.Exists {M : Type _ → Type _} [Monad M] [HHLSyntax M] {α : Type _}
+  (P : HHL.elemType M α → H.type M α) : H.type M α := fun S =>
+  --¬ HHLSyntax.Forall (fun x => ¬ P x)
+  ¬ H.Forall (fun x S => ¬ P x S) S
